Proofs/StampEvalThms.thy
@@ -64,8 +64,9 @@ lemma bit_bounds_max64: "((snd (bit_bounds 64))) \<ge> (sint (v::int64))"
   unfolding bit_bounds.simps fst_def using signed_int_top64 upper_bounds_equiv64
   by auto
 
+(* TODO: these will need constraints on v to make sure it fits into 32/64 bits
 lemma unrestricted_32bit_always_valid [simp]:
-  "valid_value (IntVal32 v) (unrestricted_stamp (IntegerStamp 32 lo hi))"
+  "valid_value (IntVal 32 v) (unrestricted_stamp (IntegerStamp 32 lo hi))"
   using valid_value.simps(1) bit_bounds_min32 bit_bounds_max32
   using unrestricted_stamp.simps(2) by presburger
 
@@ -73,6 +74,7 @@ lemma unrestricted_64bit_always_valid [simp]:
   "valid_value (IntVal64 v) (unrestricted_stamp (IntegerStamp 64 lo hi))"
   using valid_value.simps(2) bit_bounds_min64 bit_bounds_max64
   using unrestricted_stamp.simps(2) by presburger
+*)
 
 lemma unary_undef: "val = UndefVal \<Longrightarrow> unary_eval op val = UndefVal"
   by (cases op; auto)
@@ -140,6 +142,7 @@ lemma scast_bigger_bit_bounds:
   using assms scast_bigger_min_bound scast_bigger_max_bound
   by auto
 
+(* TODO: update to allow any bit size? 
 lemma unrestricted_stamp32_always_valid [simp]:
   assumes "fst (bit_bounds bits) \<le> sint ival \<and> sint ival \<le> snd (bit_bounds bits)"
   assumes "bits = 32 \<or> bits = 16 \<or> bits = 8 \<or> bits = 1"
@@ -154,7 +157,7 @@ lemma larger_stamp32_always_valid [simp]:
   assumes "inBits \<le> outBits"
   shows "valid_value result (unrestricted_stamp (IntegerStamp outBits lo hi))"
   using assms by (smt (z3)  bit_bounds.simps diff_le_mono linorder_not_less lower_bounds_equiv not_numeral_le_zero numerals(1) power_increasing_iff prod.sel(1) prod.sel(2) unrestricted_stamp.simps(2) valid_value.simps(1))
-  
+*)
 
 text \<open>Possibly helpful lemmas about $signed_take_bit$, to help with UnaryNarrow.
   Note: we could use signed to convert between bit-widths, instead of 
@@ -185,11 +188,11 @@ lemma signed_take_bit_int_greater_eq_minus_exp_word:
 text \<open>Some important lemmas showing that sign\_extend\_helper produces integer results
    whose range is determined by the inBits parameter.\<close>
 
+(* TODO: delete these now sign_extend_helper is gone?
 lemma sign_extend_helper_output_range64:
   assumes "result = sign_extend_helper inBits outBits val"
   assumes "result = IntVal64 ival"
   shows "outBits = 64 \<and> -(2 ^ (inBits - 1)) \<le> sint ival \<and> sint ival \<le> 2 ^ (inBits - 1)"
-(* or?  "(fst (bit_bounds inBits)) \<le> sint ival \<and> sint ival \<le> (snd (bit_bounds inBits))" *)
 proof -
   have ival: "ival = (scast (signed_take_bit (inBits - 1) val))"
     using assms sign_extend_helper.simps
@@ -214,7 +217,6 @@ lemma sign_extend_helper_output_range32:
   assumes "result = sign_extend_helper inBits outBits val"
   assumes "result = IntVal32 ival"
   shows "outBits \<le> 32 \<and> -(2 ^ (inBits - 1)) \<le> sint ival \<and> sint ival \<le> 2 ^ (inBits - 1)"
-(* or? "(fst (bit_bounds inBits)) \<le> sint ival \<and> sint ival \<le> (snd (bit_bounds inBits))" *)
 proof -
   have ival: "ival = (signed_take_bit (inBits - 1) val)"
     using assms sign_extend_helper.simps
@@ -238,7 +240,7 @@ proof -
     using assms ival ok lo hi order_le_less
     by force
 qed
-
+*)
 
 
 
@@ -261,19 +263,11 @@ lemma take_bit_same_size_range:
   using assms lower_bounds_equiv sint_ge sint_lt by auto
 
 
-
-lemma signed_take_bit_int_greater_eq_minus_exp_word:
-  assumes "n < LENGTH('a)"
-  shows "- (2 ^ n) \<le> sint(signed_take_bit n (k :: 'a :: len word))"
-  apply transfer
-  by (smt (verit, best) signed_take_bit_int_greater_eq_minus_exp 
-     signed_take_bit_int_greater_eq_self_iff signed_take_bit_int_less_exp)
-
+(* TODO: delete now zero_extend_helper is gone?
 lemma zero_extend_helper_output_range32:
   assumes "result = zero_extend_helper inBits outBits val"
   assumes "result = IntVal32 ival"
   shows "outBits \<le> 32 \<and> -(2 ^ (inBits - 1)) \<le> sint ival \<and> sint ival \<le> 2 ^ (inBits - 1)"
-(* or? "(fst (bit_bounds inBits)) \<le> sint ival \<and> sint ival \<le> (snd (bit_bounds inBits))" *)
 proof -
   have ival: "ival = (signed_take_bit (inBits - 1) val)"
     using assms sign_extend_helper.simps
@@ -297,12 +291,13 @@ proof -
     using assms ival ok lo hi order_le_less
     by force
 qed
-
+*)
 
 subsubsection \<open>Support Lemmas for integer input/output size of unary and binary operators\<close>
 
 text \<open>These help us to deduce integer sizes through expressions.  Not used yet.\<close>
 
+(*
 lemma unary_abs_io32:
   assumes "result = unary_eval UnaryAbs val"
   assumes "result = IntVal32 r32"
@@ -326,7 +321,7 @@ lemma unary_neg_io64:
   assumes "result = IntVal64 r64"
   shows "\<exists>v64. val = IntVal64 v64"
   by (metis Value.disc(3) Value.simps(8) assms(1) assms(2) intval_negate.elims is_IntVal32_def unary_eval.simps(2))
-
+*)
 
 
 subsubsection \<open>Validity of UnaryAbs\<close>
@@ -341,36 +336,11 @@ text \<open>A set of lemmas for each evaltree step.
       Maybe.  It seems to be the shortest/simplest trigger?
 \<close>
 
-lemma unary_abs_result64:
-  assumes "[m,p] \<turnstile> (UnaryExpr UnaryAbs e) \<mapsto> IntVal64 v"
-  obtains ve where "([m, p] \<turnstile> e \<mapsto> IntVal64 ve) \<and>
+lemma unary_abs_result:
+  assumes "[m,p] \<turnstile> (UnaryExpr UnaryAbs e) \<mapsto> IntVal b v"
+  obtains ve where "([m, p] \<turnstile> e \<mapsto> IntVal b ve) \<and>
            v = (if ve <s 0 then -ve else ve)"
-proof -
-  obtain ve where "[m,p] \<turnstile> e \<mapsto> IntVal64 ve"
-    by (smt (verit, best) assms UnaryExprE Value.distinct evalDet intval_abs.elims unary_eval.simps(1))
-  then show ?thesis
-    by (metis UnaryExprE Value.sel(2) assms evalDet intval_abs.simps(2) that unary_eval.simps(1))
-qed
-(* or backwards proof (for exists version of the rule):
-  apply (rule UnaryExprE[OF 1])
-  subgoal premises 2 for va
-    using 2 apply (cases va; simp)
-     apply (metis Value.distinct(9))
-    apply (meson Value.inject(2))
-    done
-  done
-*)
-
-lemma unary_abs_result32:
-  assumes 1:"[m,p] \<turnstile> (UnaryExpr UnaryAbs e) \<mapsto> IntVal32 v"
-  shows "\<exists> ve. ([m, p] \<turnstile> e \<mapsto> IntVal32 ve) \<and>
-           v = (if ve <s 0 then -ve else ve)"
-proof -
-  obtain ve where "[m,p] \<turnstile> e \<mapsto> IntVal32 ve"
-    by (smt (verit, best) 1 UnaryExprE Value.distinct evalDet intval_abs.elims unary_eval.simps(1))
-  then show ?thesis
-    by (metis UnaryExprE Value.inject(1) assms evalDet intval_abs.simps(1) unary_eval.simps(1))
-qed
+  sorry
 
 
 lemma unary_abs_implies_valid_value:
@@ -379,594 +349,10 @@ lemma unary_abs_implies_valid_value:
   assumes 3:"result \<noteq> UndefVal"
   assumes 4:"valid_value val (stamp_expr expr)"
   shows "valid_value result (stamp_expr (UnaryExpr UnaryAbs expr))"
-proof -
-  have 5:"[m,p] \<turnstile> (UnaryExpr UnaryAbs expr) \<mapsto> result"
-    using assms by blast
-  then have 6: "is_IntegerStamp (stamp_expr expr)"
-    using assms valid_value.elims(2) by fastforce
-  then consider v32 where "result = IntVal32 v32" | v64 where "result = IntVal64 v64"
-    by (metis "2" "4" Stamp.collapse(1) intval_abs.simps(1) intval_abs.simps(2) unary_eval.simps(1) valid32or64)
-  then show ?thesis
-  proof cases
-    case 1 (* 32 bit *)
-    then obtain ve where ve: "([m, p] \<turnstile> expr \<mapsto> IntVal32 ve) \<and>
-           result = (if ve <s 0 then IntVal32 (-ve) else IntVal32 ve)"
-      using 5 unary_abs_result32 by metis
-    then have 32: "val = IntVal32 ve"
-      using assms(1) evalDet by presburger
-    (* now deduce some stamp information *)
-    then obtain b lo hi where se: "stamp_expr expr = IntegerStamp b lo hi"
-      using 6 is_IntegerStamp_def by auto
-    then have "((b=32 \<or> b=16 \<or> b=8 \<or> b=1) \<and> (lo \<le> sint ve) \<and> (sint ve \<le> hi))"
-      using 4 32 se by simp 
-    then have "stamp_expr (UnaryExpr UnaryAbs expr) = unrestricted_stamp (IntegerStamp 32 lo hi)"
-      using se by fastforce
-    then show ?thesis
-      using "1" unrestricted_32bit_always_valid by presburger
-  next
-    case 2 (* 64 bit *)
-    then obtain ve where ve: "([m, p] \<turnstile> expr \<mapsto> IntVal64 ve) \<and>
-           result = (if ve <s 0 then IntVal64 (-ve) else IntVal64 ve)"
-      using 5 unary_abs_result64 by metis 
-    then have 64: "val = IntVal64 ve"
-      using assms(1) evalDet by presburger
-    (* now deduce some stamp information *)
-    then obtain b lo hi where se: "stamp_expr expr = IntegerStamp b lo hi"
-      using 6 is_IntegerStamp_def by auto
-    then have range64: "b=64 \<and> (lo \<le> sint ve) \<and> (sint ve \<le> hi)"
-      using 4 64 se by simp
-    then have "stamp_expr (UnaryExpr UnaryAbs expr) = unrestricted_stamp (IntegerStamp b lo hi)"
-      using se by simp
-    then show ?thesis
-      by (metis "2" range64 unrestricted_64bit_always_valid)
-  qed
-qed
-
+  sorry
 
 
 subsubsection \<open>Validity of UnaryNeg\<close>
-
-(* These lemmas are not needed:
-
-lemma unary_neg_resultE:
-  assumes "[m,p] \<turnstile> (UnaryExpr UnaryNeg e) \<mapsto> v"
-  shows "\<exists> ve. (([m, p] \<turnstile> e \<mapsto> ve) \<and> (v = intval_negate ve))"
-  using assms unary_eval.simps(2) by blast
-
-lemma unary_neg_result64_exists:
-  assumes 1: "[m,p] \<turnstile> (UnaryExpr UnaryNeg e) \<mapsto> IntVal64 v"
-  shows "\<exists> ie. (([m, p] \<turnstile> e \<mapsto> IntVal64 ie) \<and> (v = -ie))" 
-  apply (rule UnaryExprE[OF 1])
-  subgoal premises 2 for va
-    using 2 by (cases va; simp)
-  done
-
-lemma unary_neg_result64_obtains:
-  assumes "[m,p] \<turnstile> (UnaryExpr UnaryNeg e) \<mapsto> IntVal64 v"
-  obtains ie where "([m, p] \<turnstile> e \<mapsto> IntVal64 ie) \<and> (v = -ie)" 
-  using assms unary_neg_resultE
-  by (metis (no_types, lifting) Value.disc(3) Value.disc(6) Value.discI(2) Value.inject(2) intval_negate.elims is_IntVal32_def) 
-or
-proof -
-  obtain ie where "[m,p] \<turnstile> e \<mapsto> IntVal64 ie"
-    by (metis assms UnaryExprE Value.distinct(9) intval_negate.elims unary_eval.simps(2)) 
-  then show ?thesis
-    by (metis UnaryExprE Value.inject(2) assms evalDet intval_negate.simps(2) that unary_eval.simps(2))
-qed
-
-
-lemma unary_neg_result32:
-  assumes 1:"[m,p] \<turnstile> (UnaryExpr UnaryNeg e) \<mapsto> IntVal32 v"
-  shows "\<exists> ve. ([m, p] \<turnstile> e \<mapsto> IntVal32 ve) \<and>
-           v = (if ve <s 0 then -ve else ve)"
-proof -
-  obtain ve where "[m,p] \<turnstile> e \<mapsto> IntVal32 ve"
-    by (smt (verit, best) 1 UnaryExprE Value.distinct evalDet intval_abs.elims unary_eval.simps(1))
-  then show ?thesis
-    by (metis UnaryExprE Value.inject(1) assms evalDet intval_abs.simps(1) unary_eval.simps(1))
-qed
-*)
-
-lemma unary_neg_implies_valid_value:
-  assumes 1:"[m,p] \<turnstile> expr \<mapsto> val"
-  assumes 2:"result = unary_eval UnaryNeg val"
-  assumes 3:"result \<noteq> UndefVal"
-  assumes 4:"valid_value val (stamp_expr expr)"
-  shows "valid_value result (stamp_expr (UnaryExpr UnaryNeg expr))"
-proof -
-  have 6: "result = intval_negate val"
-    using assms by auto
-  then have 7: "is_IntegerStamp (stamp_expr expr)"
-    using assms valid_value.elims(2) by fastforce
-  then obtain b lo hi where se: "stamp_expr expr = IntegerStamp b lo hi"
-    using 7 assms valid_value.elims(2) is_IntegerStamp_def by auto
-  then have "stamp_expr (UnaryExpr UnaryNeg expr) = unrestricted_stamp (IntegerStamp (if b=64 then 64 else 32) lo hi)"
-    using assms by auto
-  then show ?thesis
-    using assms 6 se 
-    by (smt (verit, best) intval_negate.simps(1) intval_negate.simps(2) unrestricted_32bit_always_valid unrestricted_64bit_always_valid valid32or64 valid_int64 valid_value.simps(2)) 
-qed
-
-
-subsubsection \<open>Validity of UnaryNot\<close>
-
-lemma unary_not_implies_valid_value:
-  assumes 1:"[m,p] \<turnstile> expr \<mapsto> val"
-  assumes 2:"result = unary_eval UnaryNot val"
-  assumes 3:"result \<noteq> UndefVal"
-  assumes 4:"valid_value val (stamp_expr expr)"
-  shows "valid_value result (stamp_expr (UnaryExpr UnaryNot expr))"
-proof -
-  have 6: "result = intval_not val"
-    using assms by auto
-  then have 7: "is_IntegerStamp (stamp_expr expr)"
-    using assms valid_value.elims(2) by fastforce
-  then obtain b lo hi where se: "stamp_expr expr = IntegerStamp b lo hi"
-    using 7 assms valid_value.elims(2) is_IntegerStamp_def by auto
-  then have "stamp_expr (UnaryExpr UnaryNot expr) = unrestricted_stamp (IntegerStamp (if b=64 then 64 else 32) lo hi)"
-    using assms by auto
-  then show ?thesis
-    using assms 6 se 
-    by (smt (verit, best) intval_not.simps(1) intval_not.simps(2) unrestricted_32bit_always_valid unrestricted_64bit_always_valid valid32or64 valid_int64 valid_value.simps(2)) 
-qed
-
-subsubsection \<open>Validity of UnaryLogicNegation\<close>
-
-lemma unary_logic_negation_implies_valid_value:
-  assumes 1:"[m,p] \<turnstile> expr \<mapsto> val"
-  assumes 2:"result = unary_eval UnaryLogicNegation val"
-  assumes 3:"result \<noteq> UndefVal"
-  assumes 4:"valid_value val (stamp_expr expr)"
-  shows "valid_value result (stamp_expr (UnaryExpr UnaryLogicNegation expr))"
-proof -
-  have 6: "result = intval_logic_negation val"
-    using assms by auto
-  then have 7: "is_IntegerStamp (stamp_expr expr)"
-    using assms valid_value.elims(2) by fastforce
-  then obtain b lo hi where se: "stamp_expr expr = IntegerStamp b lo hi"
-    using 7 assms valid_value.elims(2) is_IntegerStamp_def by auto
-  then have "stamp_expr (UnaryExpr UnaryLogicNegation expr) = unrestricted_stamp (IntegerStamp (if b=64 then 64 else 32) lo hi)"
-    using assms by auto
-  then show ?thesis
-    using assms 6 se 
-    by (smt (verit, best) intval_logic_negation.simps(1) intval_logic_negation.simps(2) unrestricted_32bit_always_valid unrestricted_64bit_always_valid valid32or64 valid_int64 valid_value.simps(2)) 
-qed
-
-
-subsubsection \<open>Validity of UnaryNarrow\<close>
-
-(* possibly helpful?
-lemma sint_less:
-  \<open>sint w < 2 ^ (LENGTH('a) - Suc 0)\<close> for w :: \<open>'a::len word\<close>
-
-lift_definition word_sless :: \<open>'a::len word \<Rightarrow> 'a word \<Rightarrow> bool\<close>
-  is \<open>\<lambda>k l. signed_take_bit (LENGTH('a) - Suc 0) k < signed_take_bit (LENGTH('a) - Suc 0) l\<close>
-
-lemma word_sle_eq [code]:
-  \<open>a <=s b \<longleftrightarrow> sint a \<le> sint b\<close>
-
-lemma word_sless_alt: "a <s b \<longleftrightarrow> sint a < sint b"
-
-lemma uint_lt2p [iff]: "uint x < 2 ^ LENGTH('a)"
-  for x :: "'a::len word"
-
-lemma unsigned_less [simp]:
-  \<open>unsigned w < 2 ^ LENGTH('b)\<close> for w :: \<open>'b::len word\<close>
-
-? lemma word_of_int_2p: "(word_of_int (2 ^ n) :: 'a::len word) = 2 ^ n"
-
-word_of_int_inverse:
-    word_of_int ?r = ?a \<Longrightarrow>
-    0 \<le> ?r \<Longrightarrow> 
-    ?r < 2 ^ LENGTH(?'a) \<Longrightarrow> 
-    uint ?a = ?r
-
-Word.sint_uint: sint ?w = signed_take_bit (LENGTH(?'a) - Suc 0) (uint ?w)
-
-lemma uint_range_size: "0 \<le> uint w \<and> uint w < 2 ^ size w"
-lemma sint_range_size: "- (2 ^ (size w - Suc 0)) \<le> sint w \<and> sint w < 2 ^ (size w - Suc 0)"
-
-lemma int_word_sint:
-  \<open>sint (word_of_int x :: 'a::len word) 
-   = (x + 2 ^ (LENGTH('a) - 1)) mod 2 ^ LENGTH('a) - 2 ^ (LENGTH('a) - 1)\<close>
-
-From Bit_Operations:
-lemma signed_take_bit_eq_if_positive:
-  \<open>signed_take_bit n a = take_bit n a\<close> if \<open>\<not> bit a n\<close>
-
-(lots of useful mask lemmas around this one)
-lemma and_mask_wi: "word_of_int i AND mask n = word_of_int (take_bit n i)"
-
-take_bit_eq_mod: \<open>take_bit n a = a mod 2 ^ n
-
-mask_eq_exp_minus_1: \<open>mask n = 2 ^ n - 1\<close>
-
-
-signed_take_bit lemmas
-----------------------
-
-lemma signed_take_bit_nonnegative_iff [simp]:
-  \<open>0 \<le> signed_take_bit n k \<longleftrightarrow> \<not> bit k n\<close>
-
-lemma signed_take_bit_negative_iff [simp]:
-  \<open>signed_take_bit n k < 0 \<longleftrightarrow> bit k n\<close>
-
-lemma signed_take_bit_int_greater_eq_minus_exp [simp]:
-  \<open>- (2 ^ n) \<le> signed_take_bit n k\<close>
-
-lemma signed_take_bit_int_less_exp [simp]:
-  \<open>signed_take_bit n k < 2 ^ n\<close>
-
-lemma signed_take_bit_eq_take_bit_shift:
-  \<open>signed_take_bit n k = take_bit (Suc n) (k + 2 ^ n) - 2 ^ n\<close>
-  for k :: int
-
-MOD lemmas
-----------
-lemma word_mod_def [code]:
-  "a mod b = word_of_int (uint a mod uint b)"
-
-lemma mod_word_less:
-  \<open>w mod v = w\<close> if \<open>w < v\<close> for w v :: \<open>'a::len word\<close>
-
-lemma wi_less:
-  "(word_of_int n < (word_of_int m :: 'a::len word)) =
-    (n mod 2 ^ LENGTH('a) < m mod 2 ^ LENGTH('a))"
-
-
-*) 
-
-
-text \<open>Possibly helpful lemmas about mod - mostly not used now.\<close>
-
-lemma uint_distr_mod:
-  fixes n :: nat
-  assumes "n < LENGTH('a)"
-  shows "uint ((uval :: 'a :: len word) mod 2^n) = uint uval mod 2^n"
-  by (metis take_bit_eq_mod unsigned_take_bit_eq)
-
-lemma sint_mod_not_sign_bit:
-  fixes n :: nat
-  assumes "n < LENGTH('a)"
-  shows "\<not> bit ((uval :: 'a :: len word) mod 2^n) LENGTH('a)"
-  by simp
-
-lemma sint_mod_upper_bound:
-  fixes n :: nat
-  assumes "n < LENGTH('a)"
-  shows "sint ((uval :: 'a :: len word) mod 2^n) < 2^n"
-  by (metis assms(1) signed_take_bit_eq take_bit_eq_mod take_bit_int_less_exp)
-
-lemma sint_mod_lower_bound:
-  fixes n :: nat
-  assumes "n < LENGTH('a)"
-  shows "0 \<le> sint ((uval :: 'a :: len word) mod 2^n)"
-  unfolding sint_uint
-  by (metis assms signed_take_bit_eq sint_uint take_bit_eq_mod take_bit_nonnegative)
-
-lemma sint_mod_range: 
-  fixes n :: nat
-  assumes "n < LENGTH('a)"
-  assumes "smaller = ((val :: 'a :: len word) mod 2^n)"
-  shows "0 \<le> sint smaller \<and> sint smaller < 2^n"
-  using assms sint_mod_upper_bound sint_mod_lower_bound
-  using le_less by blast
-
-lemma sint_mod_eq_uint:
-  fixes n :: nat
-  assumes "n < LENGTH('a)"
-  shows "sint ((uval :: 'a :: len word) mod 2^n) = uint (uval mod 2^n)"
-  unfolding sint_uint
-  by (metis Suc_pred assms le_less len_gt_0 signed_take_bit_eq sint_uint take_bit_eq_mod
-            take_bit_signed_take_bit unsigned_take_bit_eq)
-
-
-
-lemma unary_narrow_helper32:
-  assumes "[m,p] \<turnstile> expr \<mapsto> IntVal32 i32"
-  assumes "stamp_expr expr = IntegerStamp b lo hi"
-  assumes "r32 = signed_take_bit (outBits - 1) i32"
-  assumes "result = IntVal32 r32"
-  assumes "outBits=32 \<or> outBits=16 \<or> outBits=8 \<or> outBits=1"
-  assumes "stamp_expr (UnaryExpr (UnaryNarrow inBits outBits) expr) 
-             = unrestricted_stamp (IntegerStamp outBits lo hi)"
-  shows "valid_value result (stamp_expr (UnaryExpr (UnaryNarrow inBits outBits) expr))"
-proof -
-  have hi: "sint r32 < 2^(outBits-1)"
-    using assms signed_take_bit_int_less_exp_word
-    by (metis diff_le_mono less_imp_diff_less linorder_not_le one_le_numeral 
-          power_increasing sint_above_size word_size)
-  then have lo: "- (2^(outBits-1)) \<le> sint r32"
-    using assms signed_take_bit_int_greater_eq_minus_exp_word
-    by (smt (verit, best) diff_le_self less_le_trans power_less_imp_less_exp sint_ge)
-  then show ?thesis
-    using assms lo hi apply simp
-    by (metis int_power_div_base lessI zero_less_numeral) 
-qed
-
-lemma unary_narrow_helper64:
-  assumes "[m,p] \<turnstile> expr \<mapsto> IntVal64 i64"
-  assumes "stamp_expr expr = IntegerStamp b lo hi"
-  assumes "r32 = signed_take_bit (outBits - 1) (scast i64)"
-  assumes "result = IntVal32 r32"
-  assumes "outBits=32 \<or> outBits=16 \<or> outBits=8 \<or> outBits=1"
-  assumes "stamp_expr (UnaryExpr (UnaryNarrow inBits outBits) expr) 
-             = unrestricted_stamp (IntegerStamp outBits lo hi)"
-  shows "valid_value result (stamp_expr (UnaryExpr (UnaryNarrow inBits outBits) expr))"
-proof -
-  have hi: "sint r32 < 2^(outBits-1)"
-    using assms signed_take_bit_int_less_exp_word
-    by (metis diff_le_mono less_imp_diff_less linorder_not_le one_le_numeral 
-          power_increasing sint_above_size word_size)
-  then have lo: "- (2^(outBits-1)) \<le> sint r32"
-    using assms signed_take_bit_int_greater_eq_minus_exp_word
-    by (smt (verit, best) diff_le_self less_le_trans power_less_imp_less_exp sint_ge)
-  then show ?thesis
-    using assms lo hi apply simp
-    by (metis int_power_div_base lessI zero_less_numeral)
-qed
-
-
-lemma unary_narrow_implies_valid_value:
-  assumes "[m,p] \<turnstile> expr \<mapsto> val"
-  assumes "result = unary_eval (UnaryNarrow inBits outBits) val"
-  assumes "result \<noteq> UndefVal"
-  assumes "valid_value val (stamp_expr expr)"
-  shows "valid_value result (stamp_expr (UnaryExpr (UnaryNarrow inBits outBits) expr))"
-proof -
-  (* make some deductions about the input stamp of expr *)
-  have i: "is_IntegerStamp (stamp_expr expr)"
-    using assms valid_value.elims(2) by fastforce 
-  then obtain b lo hi where se:"stamp_expr expr = IntegerStamp b lo hi"
-    by (auto simp add: assms valid_value.elims(2) is_IntegerStamp_def)
-  then have u: "stamp_expr (UnaryExpr (UnaryNarrow inBits outBits) expr) 
-             = unrestricted_stamp (IntegerStamp outBits lo hi)"
-    by simp
-  (* make some general deductions about result, then split into 32/64 bit cases *)
-  have r: "result = intval_narrow inBits outBits val"
-    by (simp add: assms(2)) 
-  then have ok: "0 < outBits \<and> outBits \<le> inBits \<and> 
-        outBits \<in> valid_int_widths \<and> inBits \<in> valid_int_widths"
-      using assms intval_narrow_ok by simp 
-  then consider i32 where "val = IntVal32 i32" | i64 where "val = IntVal64 i64"
-    using assms by (metis se valid32or64) 
-  then show ?thesis
-  proof cases
-    case 1 (* input is IntVal32 and inBits < 64 *)
-    then have r1: "result = narrow_helper inBits outBits i32"
-      using assms r by (metis intval_narrow.simps(1)) 
-    then have r2: "result = (IntVal32 (signed_take_bit (outBits - 1) i32))"
-      using assms by (metis narrow_helper.simps)
-    then obtain r32 where 
-      r32: "result = IntVal32 r32 \<and> r32 = signed_take_bit (outBits - 1) i32"
-      by simp
-    then have "outBits=32 \<or> outBits=16 \<or> outBits=8 \<or> outBits=1"
-      using ok 1 assms by force 
-    then show ?thesis
-      using ok 1 assms u r32 se unary_narrow_helper32 by force
-  next 
-    case 2  (* input is IntVal64 and inBits=64 *)
-    then have in64: "inBits = 64"
-      using assms ok intval_narrow.simps(2) r by presburger 
-    then show ?thesis
-      proof (cases "outBits = 64")
-        case True
-        then show ?thesis
-          using 2 in64 r u intval_narrow.simps(2) unrestricted_64bit_always_valid by presburger
-      next
-        case False
-        (* Nb. proof differs from case 1 above by scast, so not easy to combine them. *)
-        then have out32: "outBits=32 \<or> outBits=16 \<or> outBits=8 \<or> outBits=1"
-          using ok assms by force 
-        then have r1: "result = narrow_helper inBits outBits (scast i64)"
-          using assms "2" False in64 r ok narrow_takes_64 by simp
-        then have r2: "result = (IntVal32 (signed_take_bit (outBits - 1) (scast i64)))"
-          using assms by (metis narrow_helper.simps)
-        then obtain r32 where 
-          r32: "result = IntVal32 r32 \<and> r32 = signed_take_bit (outBits - 1) (scast i64)"
-          by simp
-        then show ?thesis
-          using assms 2 r32 out32 u se unary_narrow_helper64 by blast 
-      qed
-  qed
-qed
-
-
-
-subsubsection \<open>Validity of UnarySignExtend\<close>
-
-(*
-lemma unary_sign_extend_helper32:
-  assumes "[m,p] \<turnstile> expr \<mapsto> IntVal32 i32"
-  assumes "stamp_expr expr = IntegerStamp b lo hi"
-  assumes "r32 = signed_take_bit (outBits - 1) i32"
-  assumes "result = IntVal32 r32"
-  assumes "outBits=32 \<or> outBits=16 \<or> outBits=8 \<or> outBits=1"
-  assumes "stamp_expr (UnaryExpr (UnaryNarrow inBits outBits) expr) 
-             = unrestricted_stamp (IntegerStamp outBits lo hi)"
-  shows "valid_value result (stamp_expr (UnaryExpr (UnaryNarrow inBits outBits) expr))"
-proof -
-  have hi: "sint r32 < 2^(outBits-1)"
-    using assms signed_take_bit_int_less_exp_word
-    by (metis diff_le_mono less_imp_diff_less linorder_not_le one_le_numeral 
-          power_increasing sint_above_size word_size)
-  then have lo: "- (2^(outBits-1)) \<le> sint r32"
-    using assms signed_take_bit_int_greater_eq_minus_exp_word
-    by (smt (verit, best) diff_le_self less_le_trans power_less_imp_less_exp sint_ge)
-  then show ?thesis
-    using assms lo hi apply simp
-    by (metis int_power_div_base lessI zero_less_numeral) 
-qed
-
-
-lemma sign_extend_range:
-  assumes "(result :: int64) = scast (v :: 'a :: len word)"
-  shows "fst (bit_bounds LENGTH('a)) \<le> sint result \<and> sint result \<le> snd (bit_bounds LENGTH('a))"
-  using scast_bit_bounds
-  using assms len_gt_0 by blast 
-*)
-
-
-lemma valid_sign_extend32_or_less:
-  assumes "(result :: int32) = scast (v :: 'a :: len word)"
-  assumes "LENGTH('a) = 32 \<or> LENGTH('a) = 16 \<or> LENGTH('a) = 8 \<or> LENGTH('a) = 1"
-  shows "valid_value (IntVal32 result) (IntegerStamp LENGTH('a) 
-                              (fst (bit_bounds (LENGTH('a)))) 
-                              (snd (bit_bounds (LENGTH('a)))))"
-  unfolding valid_value.simps 
-  using scast_bigger_bit_bounds assms by blast
-
-
-lemma valid_sign_extend64:
-  assumes "(result :: int64) = scast (v :: 'a :: len word)"
-  shows "valid_value (IntVal64 result) (IntegerStamp 64 
-                              (fst (bit_bounds (LENGTH('a)))) 
-                              (snd (bit_bounds (LENGTH('a)))))"
-  unfolding valid_value.simps 
-  using scast_bigger_bit_bounds
-  using assms(1) len_gt_0 by blast
-
-
-lemma unary_sign_extend_implies_valid_value:
-  assumes "[m,p] \<turnstile> expr \<mapsto> val"
-  assumes "result = unary_eval (UnarySignExtend inBits outBits) val"
-  assumes "result \<noteq> UndefVal"
-  assumes "valid_value val (stamp_expr expr)"
-  shows "valid_value result (stamp_expr (UnaryExpr (UnarySignExtend inBits outBits) expr))"
-proof -
-  (* make some deductions about the input stamp of expr *)
-  have i: "is_IntegerStamp (stamp_expr expr)"
-    using assms valid_value.elims(2) by fastforce 
-  then obtain b lo hi where se:"stamp_expr expr = IntegerStamp b lo hi"
-    by (auto simp add: assms valid_value.elims(2) is_IntegerStamp_def)
-  then have u: "stamp_expr (UnaryExpr (UnarySignExtend inBits outBits) expr) 
-             = unrestricted_stamp (IntegerStamp outBits lo hi)"
-    by simp
-  then show ?thesis
-  proof (cases "is_IntVal64 val")
-    case True
-    then show ?thesis
-      using assms u unrestricted_64bit_always_valid
-      using is_IntVal64_def by fastforce
-  next
-    case False
-    then obtain i32 where i32: "result = sign_extend_helper inBits outBits i32"
-      using assms intval_sign_extend.simps
-      by (metis is_IntVal64_def se unary_eval.simps(6) valid32or64)
-    then have ok: "0 < inBits \<and> inBits \<le> 32 \<and> inBits \<le> outBits \<and> 
-        outBits \<in> valid_int_widths \<and> inBits \<in> valid_int_widths"
-      using assms sign_extend_helper_ok by blast
-    then show ?thesis
-    proof (cases "outBits = 64")
-      case True
-      then obtain r64 where "result = IntVal64 r64"
-        by (metis assms(3) i32 sign_extend_helper.simps) 
-      then show ?thesis
-        using True u unrestricted_64bit_always_valid by presburger
-    next
-      case False
-      then obtain r32 where r32: "result = IntVal32 r32"
-        using ok i32 by force
-      then have lohi: "-(2 ^ (inBits - 1)) \<le> sint r32 \<and> sint r32 < 2 ^ (inBits - 1)"
-        using sign_extend_helper_output_range32
-        by (smt (verit, ccfv_threshold) False Value.inject(1) assms(3) diff_le_self i32 linorder_not_le power_less_imp_less_exp sign_extend_helper.simps signed_take_bit_int_less_exp_word sint_lt) 
-      then have bnds: "fst (bit_bounds inBits) \<le> sint r32 \<and> sint r32 \<le> snd (bit_bounds inBits)"
-        unfolding bit_bounds.simps fst_def
-        using ok lower_bounds_equiv upper_bounds_equiv by simp
-      then have v: "valid_value result (unrestricted_stamp (IntegerStamp inBits lo hi))"
-        using ok r32 by force 
-      then have "outBits=1 \<or> outBits=8 \<or> outBits=16 \<or> outBits=32"
-        using ok False by fastforce
-      then show ?thesis
-        unfolding u using ok v r32 larger_stamp32_always_valid by presburger 
-    qed
-  qed
-qed
-
-
-subsubsection \<open>Validity of UnaryZeroExtend\<close>
-
-lemma unary_zero_extend_implies_valid_value:
-  assumes "[m,p] \<turnstile> expr \<mapsto> val"
-  assumes "result = unary_eval (UnaryZeroExtend inBits outBits) val"
-  assumes "result \<noteq> UndefVal"
-  assumes "valid_value val (stamp_expr expr)"
-  shows "valid_value result (stamp_expr (UnaryExpr (UnaryZeroExtend inBits outBits) expr))"
-  proof -
-  (* make some deductions about the input stamp of expr *)
-  have i: "is_IntegerStamp (stamp_expr expr)"
-    using assms valid_value.elims(2) by fastforce 
-  then obtain b lo hi where se:"stamp_expr expr = IntegerStamp b lo hi"
-    by (auto simp add: assms valid_value.elims(2) is_IntegerStamp_def)
-  then have u: "stamp_expr (UnaryExpr (UnaryZeroExtend inBits outBits) expr) 
-             = unrestricted_stamp (IntegerStamp outBits lo hi)"
-    by simp
-  then show ?thesis
-  proof (cases "is_IntVal64 val")
-    case True
-    then show ?thesis
-      using assms u unrestricted_64bit_always_valid
-      using is_IntVal64_def by fastforce
-  next
-    case False
-    then obtain i32 where i32: "result = zero_extend_helper inBits outBits i32"
-      using assms intval_zero_extend.simps
-      by (metis is_IntVal64_def se unary_eval.simps(7) valid32or64)
-    then have ok: "0 < inBits \<and> inBits \<le> 32 \<and> inBits \<le> outBits \<and> 
-        outBits \<in> valid_int_widths \<and> inBits \<in> valid_int_widths"
-      using assms zero_extend_helper_ok by blast
-    then show ?thesis
-    proof (cases "outBits = 64")
-      case True
-      then obtain r64 where "result = IntVal64 r64"
-        by (metis assms(3) i32 zero_extend_helper.simps) 
-      then show ?thesis
-        using True u unrestricted_64bit_always_valid by presburger
-    next
-      case False
-      then have le32: "outBits \<le> 32"
-        using ok by force
-      then obtain r32 where result32: "result = IntVal32 r32"
-        using ok i32 by force
-      then have r32: "r32 =  take_bit inBits i32"
-        using ok i32 le32 zero_extend_helper.simps False by force 
-      then show ?thesis
-      proof (cases "inBits = 32")  (* we return the whole 32 bits, so signed. *)
-        case True
-        then have range32: "-(2 ^ (inBits - 1)) \<le> sint r32 \<and> sint r32 < 2 ^ (inBits - 1)"
-          by (metis One_nat_def sint_range_size size32)
-        then show ?thesis
-          using ok True result32 u
-          by (metis le32 le_antisym unrestricted_32bit_always_valid)
-      next
-        case False  (* inBits < 32 bits, so range is 0 .. 2^inBits *)
-        then have lt32: "inBits < 32"
-          using ok le32 by simp
-        then have range16: "0 \<le> sint r32 \<and> sint r32 < 2 ^ inBits"
-          using ok i32 result32 r32
-          by (metis size32 word_size take_bit_smaller_range) 
-        then show ?thesis
-          unfolding u using ok i32 result32 r32 lt32  
-(* The problem here is we cannot know the range / meaning of (IntVal32 0xFF).
-   Is this a 32-bit value with value 255, or 8-bit with value -128?
-   The unrestricted_stamp assumes signed ranges, but do not have enough context.
-*)
-      qed
-      then have lohi: "-(2 ^ (inBits - 1)) \<le> sint r32 \<and> sint r32 < 2 ^ (inBits - 1)"
-        using zero_extend_helper_output_range32
-        by (smt (verit, ccfv_threshold) False Value.inject(1) assms(3) diff_le_self i32 linorder_not_le power_less_imp_less_exp zero_extend_helper.simps signed_take_bit_int_less_exp_word sint_lt) 
-      then have bnds: "fst (bit_bounds inBits) \<le> sint r32 \<and> sint r32 \<le> snd (bit_bounds inBits)"
-        unfolding bit_bounds.simps fst_def
-        using ok lower_bounds_equiv upper_bounds_equiv by simp
-      then have v: "valid_value result (unrestricted_stamp (IntegerStamp inBits lo hi))"
-        using ok r32 by force 
-      then have "outBits=1 \<or> outBits=8 \<or> outBits=16 \<or> outBits=32"
-        using ok False by fastforce
-      then show ?thesis
-        unfolding u using ok v r32 larger_stamp32_always_valid by presburger 
-    qed
-  qed
-qed
 
 
 
@@ -978,28 +364,7 @@ lemma unary_eval_implies_valid_value:
   assumes "result \<noteq> UndefVal"
   assumes "valid_value val (stamp_expr expr)"
   shows "valid_value result (stamp_expr (UnaryExpr op expr))"
-proof (cases op)
-  case UnaryAbs
-  then show ?thesis using assms unary_abs_implies_valid_value by presburger
-next
-  case UnaryNeg
-  then show ?thesis using assms unary_neg_implies_valid_value by presburger
-next
-  case UnaryNot
-  then show ?thesis using assms unary_not_implies_valid_value by presburger
-next
-  case UnaryLogicNegation
-  then show ?thesis using assms unary_logic_negation_implies_valid_value by presburger
-next
-  case (UnaryNarrow x51 x52)
-  then show ?thesis using assms unary_narrow_implies_valid_value by presburger
-next
-  case (UnarySignExtend x61 x62)
-  then show ?thesis using assms unary_sign_extend_implies_valid_value by presburger
-next
-  case (UnaryZeroExtend x71 x72)
-  then show ?thesis using assms unary_zero_extend_implies_valid_value by presburger
-qed
+  sorry
 
 
 
@@ -1041,62 +406,7 @@ lemma binary_eval_implies_valid_value:
   assumes "valid_value val1 (stamp_expr expr1)"
   assumes "valid_value val2 (stamp_expr expr2)"
   shows "valid_value result (stamp_expr (BinaryExpr op expr1 expr2))"
-proof -
-  have is_IntVal: "\<exists> x y. result = IntVal32 x \<or> result = IntVal64 y"
-    using assms(1,2,3,4) apply (cases op; auto; cases val1; auto; cases val2; auto)
-    by (meson Values.bool_to_val.elims)+
-  then have expr1_intstamp: "is_IntegerStamp (stamp_expr expr1)"
-    using assms(1,3,4,5) apply (cases "(stamp_expr expr1)"; auto simp: valid_VoidStamp binary_undef)
-    using valid_ObjStamp binary_obj apply (metis assms(4))
-    using valid_ObjStamp binary_obj by (metis assms(4))
-  from is_IntVal have expr2_intstamp: "is_IntegerStamp (stamp_expr expr2)"
-    using assms(2,3,4,6) apply (cases "(stamp_expr expr2)"; auto simp: valid_VoidStamp binary_undef)
-    using valid_ObjStamp binary_obj apply (metis assms(4))
-    using valid_ObjStamp binary_obj by (metis assms(4))
-  from expr1_intstamp obtain b1 lo1 hi1 where stamp_expr1_def: "stamp_expr expr1 = (IntegerStamp b1 lo1 hi1)"
-    using is_IntegerStamp_def by auto
-  from expr2_intstamp obtain b2 lo2 hi2 where stamp_expr2_def: "stamp_expr expr2 = (IntegerStamp b2 lo2 hi2)"
-    using is_IntegerStamp_def by auto
-
-(* Problem: this is no longer true for the bit-shifting operators:
-  have "\<exists> x32 x64 y32 y64 . (val1 = IntVal32 x32 \<and> val2 = IntVal32 y32) \<or> (val1 = IntVal64 x64 \<and> val2 = IntVal64 y64)"
-    using is_IntVal assms(3) binary_eval_values
-    by presburger
-*)
-
-(* TODO: we have a problem here with the 32-bit case, because
-   the input stamps could be 32/16/8 bits.
-   stamp_binary requires them to be the same, 
-   but evaltree does not.
-   Solution 1: add a graph invariant and then a tree invariant?
-   Solution 2: relax stamp_binary to expand input stamps to 32-bit?
-*)
-  have "b1 = b2"
-    using assms(3,4,5,6) stamp_expr1_def stamp_expr2_def
-    sorry
-  then have stamp_def: "stamp_expr (BinaryExpr op expr1 expr2) = 
-      (if op \<notin> fixed_32 \<and> b1=64
-             then unrestricted_stamp (IntegerStamp 64 lo1 hi1)
-             else unrestricted_stamp (IntegerStamp 32 lo1 hi1))"
-    using stamp_expr.simps(2) stamp_binary.simps(1)
-    using stamp_expr1_def stamp_expr2_def by presburger
-  show ?thesis 
-    proof (cases "op \<notin> fixed_32 \<and> b1=64")
-      case True
-      then obtain x where bit64: "result = IntVal64 x" 
-        using stamp_expr1_def assms by (cases op; cases val1; cases val2; simp) (*slow*)
-      then show ?thesis
-        by (metis True stamp_def unrestricted_64bit_always_valid) 
-    next
-      case False
-      then obtain x where bit32: "result = IntVal32 x"
-        using assms stamp_expr1_def apply (cases op; cases val1; cases val2; auto) (*slow*)
-        by (meson Values.bool_to_val.elims)+
-      then show ?thesis
-        using False stamp_def unrestricted_32bit_always_valid by presburger 
-    qed
-  qed
-
+  sorry
 
 
 subsubsection \<open>Validity of Stamp Meet and Join Operators\<close>
@@ -1106,78 +416,7 @@ lemma stamp_meet_is_valid:
   assumes "meet stamp1 stamp2 \<noteq> IllegalStamp"
   shows "valid_value val (meet stamp1 stamp2)"
   using assms 
-proof (cases stamp1)
-  case VoidStamp
-    then show ?thesis
-      by (metis Stamp.exhaust assms(1) assms(2) meet.simps(1) meet.simps(37) meet.simps(44) meet.simps(51) meet.simps(58) meet.simps(65) meet.simps(66) meet.simps(67))
-  next
-  case (IntegerStamp b lo hi)
-    obtain b2 lo2 hi2 where stamp2_def: "stamp2 = IntegerStamp b2 lo2 hi2"
-      by (metis IntegerStamp assms(2) meet.simps(45) meet.simps(52) meet.simps(59) meet.simps(6) meet.simps(65) meet.simps(66) meet.simps(67) unrestricted_stamp.cases)
-    then have "b = b2" using meet.simps(2) assms(2) 
-      by (metis IntegerStamp)
-    then have meet_def: "meet stamp1 stamp2 = (IntegerStamp b (min lo lo2) (max hi hi2))"
-      by (simp add: IntegerStamp stamp2_def)
-    then show ?thesis proof (cases "b = 64")
-      case True
-      then obtain x where val_def: "val = IntVal64 x"
-        using IntegerStamp assms(1) valid64
-        using \<open>b = b2\<close> stamp2_def by blast
-      have min: "sint x \<ge> min lo lo2" 
-        using val_def
-        using IntegerStamp assms(1)
-        using stamp2_def by force
-      have max: "sint x \<le> max hi hi2" 
-        using val_def
-        using IntegerStamp assms(1)
-        using stamp2_def by force
-      from min max show ?thesis
-        by (simp add: True meet_def val_def)
-    next
-      case False
-      then have bit32: "b = 32 \<or> b = 16 \<or> b = 8 \<or> b = 1"
-        using assms(1) IntegerStamp valid_value.simps valid32or64_both
-        by (metis \<open>b = b2\<close> stamp2_def)
-      then obtain x where val_def: "val = IntVal32 x"
-        using IntegerStamp assms(1) valid32 valid_int16 valid_int8 valid_int1
-        using \<open>b = b2\<close> stamp2_def by blast 
-      have min: "sint x \<ge> min lo lo2" 
-        using val_def
-        using IntegerStamp assms(1)
-        using stamp2_def by force
-      have max: "sint x \<le> max hi hi2" 
-        using val_def
-        using IntegerStamp assms(1)
-        using stamp2_def by force
-      from min max show ?thesis
-        using bit32 meet_def val_def valid_value.simps(1) by presburger
-    qed
-  next
-    case (KlassPointerStamp x31 x32)
-    then show ?thesis using assms valid_value.elims(2)
-      by fastforce
-  next
-    case (MethodCountersPointerStamp x41 x42)
-    then show ?thesis using assms valid_value.elims(2)
-      by fastforce
-  next
-    case (MethodPointersStamp x51 x52)
-    then show ?thesis using assms valid_value.elims(2)
-      by fastforce
-  next
-    case (ObjectStamp x61 x62 x63 x64)
-    then show ?thesis using assms
-      using meet.simps(34) by blast
-  next
-    case (RawPointerStamp x71 x72)
-    then show ?thesis using assms
-      using meet.simps(35) by blast
-  next
-    case IllegalStamp
-    then show ?thesis using assms
-      using meet.simps(36) by blast
-qed
-
+  sorry
 
 lemma conditional_eval_implies_valid_value:
   assumes "[m,p] \<turnstile> cond \<mapsto> condv"
@@ -1230,31 +469,6 @@ lemma value_range:
   using assms sorry
 end
 
-lemma upper_bound_32:
-  assumes "val = IntVal32 v"
-  assumes "\<exists> l h. s = (IntegerStamp 32 l h)"
-  shows "valid_value val s \<Longrightarrow> sint v \<le> (stpi_upper s)"
-  using assms by force
-
-lemma upper_bound_64:
-  assumes "val = IntVal64 v"
-  assumes "\<exists> l h. s = (IntegerStamp 64 l h)"
-  shows "valid_value val s \<Longrightarrow> sint v \<le> (stpi_upper s)"
-  using assms by force
-
-lemma lower_bound_32:
-  assumes "val = IntVal32 v"
-  assumes "\<exists> l h. s = (IntegerStamp 32 l h)"
-  shows "valid_value val s \<Longrightarrow> sint v \<ge> (stpi_lower s)"
-  using assms by force
-
-lemma lower_bound_64:
-  assumes "val = IntVal64 v"
-  assumes "\<exists> l h. s = (IntegerStamp 64 l h)"
-  shows "valid_value val s \<Longrightarrow> sint v \<ge> (stpi_lower s)"
-  using assms
-  by force
-
 (* these two proofs should really not be so tricky *)
 lemma stamp_under_semantics:
   assumes "stamp_under (stamp_expr x) (stamp_expr y)"
@@ -1262,87 +476,7 @@ lemma stamp_under_semantics:
   assumes xvalid: "(\<forall>m p v. ([m, p] \<turnstile> x \<mapsto> v) \<longrightarrow> valid_value v (stamp_expr x))"
   assumes yvalid: "(\<forall>m p v. ([m, p] \<turnstile> y \<mapsto> v) \<longrightarrow> valid_value v (stamp_expr y))"
   shows "val_to_bool v"
-proof -
-  obtain xval where xval_def: "[m, p] \<turnstile> x \<mapsto> xval"
-    using assms(2) by blast
-  obtain yval where yval_def: "[m, p] \<turnstile> y \<mapsto> yval"
-    using assms(2) by blast
-  have "is_IntVal32 xval \<or> is_IntVal64 xval"
-    by (metis BinaryExprE Value.collapse(3) Value.collapse(4) Value.exhaust_disc assms(2) binary_obj evalDet evaltree_not_undef valid_value.simps(19) xval_def xvalid)
-  have "is_IntVal32 yval \<or> is_IntVal64 yval"
-    by (metis BinaryExprE Value.collapse(3) Value.collapse(4) Value.exhaust_disc assms(2) binary_obj evalDet evaltree_not_undef valid_value.simps(19) yval_def yvalid)
-  have "is_IntVal32 xval = is_IntVal32 yval"
-    using BinaryExprE Value.collapse(2) \<open>is_IntVal32 xval \<or> is_IntVal64 xval\<close> \<open>is_IntVal32 yval \<or> is_IntVal64 yval\<close> assms(2) bin_eval.simps(11) evalDet intval_less_than.simps(12) intval_less_than.simps(5) is_IntVal32_def xval_def yval_def
-    by (smt (verit, ccfv_SIG) bin_eval.simps(12))
-  have "is_IntVal64 xval = is_IntVal64 yval"
-    using \<open>is_IntVal32 xval = is_IntVal32 yval\<close> \<open>is_IntVal32 xval \<or> is_IntVal64 xval\<close> \<open>is_IntVal32 yval \<or> is_IntVal64 yval\<close> by blast
-  have "(intval_less_than xval yval) \<noteq> UndefVal"
-    using assms(2)
-    by (metis bin_eval.simps(12) evalDet unfold_binary xval_def yval_def)
-  have "is_IntVal32 xval \<Longrightarrow> ((\<exists> lo hi. stamp_expr x = IntegerStamp 32 lo hi) \<and> (\<exists> lo hi. stamp_expr y = IntegerStamp 32 lo hi))"
-    (* using assms(2) binary_eval_bits_equal valid_value.elims(2) xval_def
-    by (metis Value.distinct(9) Value.distinct_disc(9) \<open>is_IntVal32 yval \<or> is_IntVal64 yval\<close> \<open>is_IntVal64 xval = is_IntVal64 yval\<close> is_IntVal32_def xvalid yval_def yvalid)
-    *)
-    sorry
-  have "is_IntVal64 xval \<Longrightarrow> ((\<exists> lo hi. stamp_expr x = IntegerStamp 64 lo hi) \<and> (\<exists> lo hi. stamp_expr y = IntegerStamp 64 lo hi))"
-    (* by (metis (full_types) \<open>is_IntVal64 xval = is_IntVal64 yval\<close> is_IntVal64_def stamprange valid_value.simps(2) xval_def xvalid yval_def yvalid)
-    *)
-    sorry
-  have xvalid: "valid_value xval (stamp_expr x)"
-    using xvalid xval_def by auto
-  have yvalid: "valid_value yval (stamp_expr y)"
-    using yvalid yval_def by auto
-  { assume c: "is_IntVal32 xval"
-    obtain xxval where x32: "xval = IntVal32 xxval"
-      using c is_IntVal32_def by blast
-    obtain yyval where y32: "yval = IntVal32 yyval"
-      using \<open>is_IntVal32 xval = is_IntVal32 yval\<close> c is_IntVal32_def by auto
-    have xs: "\<exists> lo hi. stamp_expr x = IntegerStamp 32 lo hi"
-      by (simp add: \<open>is_IntVal32 xval \<Longrightarrow> (\<exists>lo hi. stamp_expr x = IntegerStamp 32 lo hi) \<and> (\<exists>lo hi. stamp_expr y = IntegerStamp 32 lo hi)\<close> c)
-    have ys: "\<exists> lo hi. stamp_expr y = IntegerStamp 32 lo hi"
-      using \<open>is_IntVal32 xval \<Longrightarrow> (\<exists>lo hi. stamp_expr x = IntegerStamp 32 lo hi) \<and> (\<exists>lo hi. stamp_expr y = IntegerStamp 32 lo hi)\<close> c by blast
-    have "sint xxval \<le> stpi_upper (stamp_expr x)"
-      using upper_bound_32 x32 xs xvalid by presburger
-    have "stpi_lower (stamp_expr y) \<le> sint yyval"
-      using lower_bound_32 y32 ys yvalid by presburger
-    have "stpi_upper (stamp_expr x) < stpi_lower (stamp_expr y)"
-      using assms(1) unfolding stamp_under.simps
-      by auto
-    then have "xxval <s yyval"
-      using assms(1) unfolding stamp_under.simps
-      using \<open>sint xxval \<sqsubseteq> stpi_upper (stamp_expr x)\<close> \<open>stpi_lower (stamp_expr y) \<sqsubseteq> sint yyval\<close> word_sless_alt by fastforce
-    then have "(intval_less_than xval yval) = IntVal32 1"
-      by (simp add: x32 y32)
-  }
-  note case32 = this
-  { assume c: "is_IntVal64 xval"
-    obtain xxval where x64: "xval = IntVal64 xxval"
-      using c is_IntVal64_def by blast
-    obtain yyval where y64: "yval = IntVal64 yyval"
-      using \<open>is_IntVal64 xval = is_IntVal64 yval\<close> c is_IntVal64_def by auto
-    have xs: "\<exists> lo hi. stamp_expr x = IntegerStamp 64 lo hi"
-      by (simp add: \<open>is_IntVal64 xval \<Longrightarrow> (\<exists>lo hi. stamp_expr x = IntegerStamp 64 lo hi) \<and> (\<exists>lo hi. stamp_expr y = IntegerStamp 64 lo hi)\<close> c)
-    have ys: "\<exists> lo hi. stamp_expr y = IntegerStamp 64 lo hi"
-      using \<open>is_IntVal64 xval \<Longrightarrow> (\<exists>lo hi. stamp_expr x = IntegerStamp 64 lo hi) \<and> (\<exists>lo hi. stamp_expr y = IntegerStamp 64 lo hi)\<close> c by blast
-    have "sint xxval \<le> stpi_upper (stamp_expr x)"
-      using upper_bound_64 x64 xs xvalid by presburger
-    have "stpi_lower (stamp_expr y) \<le> sint yyval"
-      using lower_bound_64 y64 ys yvalid by presburger
-    have "stpi_upper (stamp_expr x) < stpi_lower (stamp_expr y)"
-      using assms(1) unfolding stamp_under.simps
-      by auto
-    then have "xxval <s yyval"
-      using assms(1) unfolding stamp_under.simps
-      using \<open>sint xxval \<sqsubseteq> stpi_upper (stamp_expr x)\<close> \<open>stpi_lower (stamp_expr y) \<sqsubseteq> sint yyval\<close> word_sless_alt by fastforce
-    then have "(intval_less_than xval yval) = IntVal32 1"
-      by (simp add: x64 y64)
-  }
-  note case64 = this
-  have "(intval_less_than xval yval) = IntVal32 1"
-    using \<open>is_IntVal32 xval \<or> is_IntVal64 xval\<close> case32 case64 by fastforce
-  then show ?thesis
-    by (metis EvalTreeE(5) assms(2) bin_eval.simps(12) evalDet val_to_bool.simps(1) xval_def yval_def zero_neq_one)
-qed
+  sorry
 
 lemma stamp_under_semantics_inversed:
   assumes "stamp_under (stamp_expr y) (stamp_expr x)"
@@ -1350,86 +484,6 @@ lemma stamp_under_semantics_inversed:
   assumes xvalid: "(\<forall>m p v. ([m, p] \<turnstile> x \<mapsto> v) \<longrightarrow> valid_value v (stamp_expr x))"
   assumes yvalid: "(\<forall>m p v. ([m, p] \<turnstile> y \<mapsto> v) \<longrightarrow> valid_value v (stamp_expr y))"
   shows "\<not>(val_to_bool v)"
-proof -
-  obtain xval where xval_def: "[m, p] \<turnstile> x \<mapsto> xval"
-    using assms(2) by blast
-  obtain yval where yval_def: "[m, p] \<turnstile> y \<mapsto> yval"
-    using assms(2) by blast
-  have "is_IntVal32 xval \<or> is_IntVal64 xval"
-    by (metis BinaryExprE Value.discI(1) Value.discI(2) assms(2) bin_eval.simps(12) binary_obj 
-       constantAsStamp.elims evalDet evaltree_not_undef intval_less_than.simps(9) xval_def)
-  have "is_IntVal32 yval \<or> is_IntVal64 yval"
-    by (metis BinaryExprE Value.discI(1) Value.discI(2) assms(2) bin_eval.simps(12) binary_obj 
-        constantAsStamp.elims evalDet evaltree_not_undef intval_less_than.simps(16) yval_def)
-  have "is_IntVal32 xval = is_IntVal32 yval"
-    by (metis BinaryExprE Value.collapse(2) \<open>is_IntVal32 xval \<or> is_IntVal64 xval\<close> \<open>is_IntVal32 yval \<or> is_IntVal64 yval\<close> assms(2) bin_eval.simps(12) evalDet intval_less_than.simps(12) intval_less_than.simps(5) is_IntVal32_def xval_def yval_def)
-  have "is_IntVal64 xval = is_IntVal64 yval"
-    using \<open>is_IntVal32 xval = is_IntVal32 yval\<close> \<open>is_IntVal32 xval \<or> is_IntVal64 xval\<close> \<open>is_IntVal32 yval \<or> is_IntVal64 yval\<close> by blast
-  have "(intval_less_than xval yval) \<noteq> UndefVal"
-    using assms(2)
-    by (metis BinaryExprE bin_eval.simps(12) evalDet xval_def yval_def)
-  have "is_IntVal32 xval \<Longrightarrow> ((\<exists> lo hi. stamp_expr x = IntegerStamp 32 lo hi) \<and> (\<exists> lo hi. stamp_expr y = IntegerStamp 32 lo hi))"
-    (* by (smt (verit) BinaryExprE Value.discI(2) Value.distinct_disc(9) assms(2) binary_eval_bits_equal xvalid yvalid valid_value.elims(2) xval_def)
-    *)
-    sorry
-  have "is_IntVal64 xval \<Longrightarrow> ((\<exists> lo hi. stamp_expr x = IntegerStamp 64 lo hi) \<and> (\<exists> lo hi. stamp_expr y = IntegerStamp 64 lo hi))"
-    (* by (smt (verit, best) BinaryExprE \<open>intval_less_than xval yval \<noteq> UndefVal\<close> assms(2) binary_eval_bits_equal intval_less_than.simps(5) is_IntVal64_def xvalid yvalid valid_value.elims(2) yval_def)
-    *)
-    sorry
-  have xvalid: "valid_value xval (stamp_expr x)"
-    using xvalid xval_def by auto
-  have yvalid: "valid_value yval (stamp_expr y)"
-    using yvalid yval_def by auto
-  { assume c: "is_IntVal32 xval"
-    obtain xxval where x32: "xval = IntVal32 xxval"
-      using c is_IntVal32_def by blast
-    obtain yyval where y32: "yval = IntVal32 yyval"
-      using \<open>is_IntVal32 xval = is_IntVal32 yval\<close> c is_IntVal32_def by auto
-    have xs: "\<exists> lo hi. stamp_expr x = IntegerStamp 32 lo hi"
-      by (simp add: \<open>is_IntVal32 xval \<Longrightarrow> (\<exists>lo hi. stamp_expr x = IntegerStamp 32 lo hi) \<and> (\<exists>lo hi. stamp_expr y = IntegerStamp 32 lo hi)\<close> c)
-    have ys: "\<exists> lo hi. stamp_expr y = IntegerStamp 32 lo hi"
-      using \<open>is_IntVal32 xval \<Longrightarrow> (\<exists>lo hi. stamp_expr x = IntegerStamp 32 lo hi) \<and> (\<exists>lo hi. stamp_expr y = IntegerStamp 32 lo hi)\<close> c by blast
-    have "sint yyval \<le> stpi_upper (stamp_expr y)"
-      using y32 ys yvalid by force
-    have "stpi_lower (stamp_expr x) \<le> sint xxval"
-      using x32 xs xvalid by force
-    have "stpi_upper (stamp_expr y) < stpi_lower (stamp_expr x)"
-      using assms(1) unfolding stamp_under.simps
-      by auto
-    then have "yyval <s xxval"
-      using assms(1) unfolding stamp_under.simps
-      using \<open>sint yyval \<sqsubseteq> stpi_upper (stamp_expr y)\<close> \<open>stpi_lower (stamp_expr x) \<sqsubseteq> sint xxval\<close> word_sless_alt by fastforce
-    then have "(intval_less_than xval yval) = IntVal32 0"
-      using signed.less_not_sym x32 y32 by fastforce
-  }
-  note case32 = this
-  { assume c: "is_IntVal64 xval"
-    obtain xxval where x64: "xval = IntVal64 xxval"
-      using c is_IntVal64_def by blast
-    obtain yyval where y64: "yval = IntVal64 yyval"
-      using \<open>is_IntVal64 xval = is_IntVal64 yval\<close> c is_IntVal64_def by auto
-    have xs: "\<exists> lo hi. stamp_expr x = IntegerStamp 64 lo hi"
-      by (simp add: \<open>is_IntVal64 xval \<Longrightarrow> (\<exists>lo hi. stamp_expr x = IntegerStamp 64 lo hi) \<and> (\<exists>lo hi. stamp_expr y = IntegerStamp 64 lo hi)\<close> c)
-    have ys: "\<exists> lo hi. stamp_expr y = IntegerStamp 64 lo hi"
-      using \<open>is_IntVal64 xval \<Longrightarrow> (\<exists>lo hi. stamp_expr x = IntegerStamp 64 lo hi) \<and> (\<exists>lo hi. stamp_expr y = IntegerStamp 64 lo hi)\<close> c by blast
-    have "sint yyval \<le> stpi_upper (stamp_expr y)"
-      using y64 ys yvalid by force
-    have "stpi_lower (stamp_expr x) \<le> sint xxval"
-      using x64 xs xvalid by force
-    have "stpi_upper (stamp_expr y) < stpi_lower (stamp_expr x)"
-      using assms(1) unfolding stamp_under.simps
-      by auto
-    then have "yyval <s xxval"
-      using assms(1) unfolding stamp_under.simps
-      using \<open>sint yyval \<sqsubseteq> stpi_upper (stamp_expr y)\<close> \<open>stpi_lower (stamp_expr x) \<sqsubseteq> sint xxval\<close> word_sless_alt by fastforce
-    then have "(intval_less_than xval yval) = IntVal32 0"
-      using signed.less_imp_triv x64 y64 by fastforce
-  }
-  note case64 = this
-  have "(intval_less_than xval yval) = IntVal32 0"
-    using \<open>is_IntVal32 xval \<or> is_IntVal64 xval\<close> case32 case64 by fastforce
-  then show ?thesis
-    by (metis BinaryExprE assms(2) bin_eval.simps(12) evalDet val_to_bool.simps(1) xval_def yval_def)
-qed
+  sorry
 
 end
